more

Weidenbach_Book/Watched_Literals_Algorithm_Restart.thy
@@ -48,8 +48,7 @@ definition cdcl_twl_stgy_restart_prog :: "'v twl_st \<Rightarrow> 'v twl_st nres
     RETURN T
   }\<close>
 
-lemma (in twl_restart) restart_prog_spec:
-  fixes n :: string
+lemma (in twl_restart) 
   assumes
     inv: \<open>case (brk, T, m) of  (brk, T, m) \<Rightarrow> cdcl_twl_stgy_restart_prog_inv S brk T m\<close> and
     cond: \<open>case (brk, T, m) of (brk, uu_) \<Rightarrow> \<not> brk\<close> and
@@ -59,7 +58,8 @@ lemma (in twl_restart) restart_prog_spec:
     lits_to_update: \<open>literals_to_update S' = {#}\<close> and
     \<open>\<forall>S'a. \<not> cdcl_twl_cp S' S'a\<close> and
     \<open>twl_stgy_invs S'\<close>
-  shows \<open>restart_prog U m brk'
+  shows restart_prog_spec:
+    \<open>restart_prog U m brk'
          \<le> SPEC
              (\<lambda>x. (case x of
                    (T, na) \<Rightarrow> RETURN (brk', T, na))
@@ -78,7 +78,7 @@ lemma (in twl_restart) restart_prog_spec:
      twl_struct_invs S \<and>
      cdcl_twl_stgy_restart_with_leftovers1 (S, m)
       (T, n)} \<union>
-    {((brkT, T), brkS, S). S = T \<and> brkT \<and> \<not> brkS}))\<close>
+    {((brkT, T), brkS, S). S = T \<and> brkT \<and> \<not> brkS}))\<close> (is ?A)
 proof -
   have struct_invs': \<open>cdcl_twl_restart U T \<Longrightarrow> twl_struct_invs T\<close> for T
     using assms(3) cdcl_twl_restart_twl_struct_invs by blast
@@ -233,7 +233,7 @@ proof -
 
   have [simp]: \<open>brk = False\<close>
     using cond by auto
-  show ?thesis
+  show ?A
     unfolding restart_prog_def restart_required_def
     apply (refine_vcg; remove_dummy_vars)
     subgoal using struct_invs_U stgy_invs_U confl_U unfolding restart_prog_pre_def by fast
@@ -260,6 +260,220 @@ proof -
           cdcl_twl_stgy_restart_with_leftovers_after_restart_T_V struct_invs_U
           rtranclp_twl_restart_after_restart_brk rtranclp_twl_restart_after_restart_T_U
           cdcl_twl_stgy_restart_with_leftovers1_after_restart)
+    done
+qed
+
+lemma (in twl_restart) 
+  assumes
+    inv: \<open>case (ebrk, brk, T, m) of  (ebrk, brk, T, m) \<Rightarrow> cdcl_twl_stgy_restart_prog_inv S brk T m\<close> and
+    cond: \<open>case (ebrk, brk, T, m) of (ebrk, brk, _) \<Rightarrow> \<not> brk \<and> \<not>ebrk\<close> and
+    other_inv: \<open>cdcl_twl_o_prog_spec S' (brk', U)\<close> and
+    struct_invs_S: \<open>twl_struct_invs S'\<close> and
+    cp: \<open>cdcl_twl_cp\<^sup>*\<^sup>* T S'\<close> and
+    lits_to_update: \<open>literals_to_update S' = {#}\<close> and
+    \<open>\<forall>S'a. \<not> cdcl_twl_cp S' S'a\<close> and
+    \<open>twl_stgy_invs S'\<close>
+  shows restart_prog_early_spec:
+   \<open>restart_prog U m brk'
+    \<le> SPEC
+       (\<lambda>x. (case x of (T, n) \<Rightarrow> RES UNIV \<bind> (\<lambda>ebrk. RETURN (ebrk, brk', T, n)))
+            \<le> SPEC
+               (\<lambda>s'. (case s' of (ebrk, brk, x, xb) \<Rightarrow>
+                        cdcl_twl_stgy_restart_prog_inv S brk x xb) \<and>
+                     (s', ebrk, brk, T, m)
+                     \<in> {((ebrk, brkT, T, n), ebrk, brkS, S, m).
+                        twl_struct_invs S \<and>
+                        cdcl_twl_stgy_restart_with_leftovers1 (S, m) (T, n)} \<union>
+                       {((ebrkT, brkT, T), ebrkS, brkS, S).
+                           S = T \<and> (ebrkT \<or> brkT) \<and> \<not> brkS \<and> \<not> ebrkS}))\<close>  (is \<open>?B\<close>)
+proof -
+  have struct_invs': \<open>cdcl_twl_restart U T \<Longrightarrow> twl_struct_invs T\<close> for T
+    using assms(3) cdcl_twl_restart_twl_struct_invs by blast
+  have stgy_invs: \<open>cdcl_twl_restart U V \<Longrightarrow>twl_stgy_invs V\<close> for V
+    using assms(3) cdcl_twl_restart_twl_stgy_invs by blast
+  have res_no_clss_to_upd: \<open>cdcl_twl_restart U V \<Longrightarrow> clauses_to_update V = {#}\<close> for V
+    by (auto simp: cdcl_twl_restart.simps)
+  have res_no_confl: \<open>cdcl_twl_restart U V \<Longrightarrow> get_conflict V = None\<close> for V
+    by (auto simp: cdcl_twl_restart.simps)
+
+  have
+    struct_invs_T: \<open>twl_struct_invs T\<close> and
+    \<open>twl_stgy_invs T\<close> and
+    \<open>brk \<longrightarrow> final_twl_state T\<close> and
+    twl_res: \<open>cdcl_twl_stgy_restart_with_leftovers (S, 0) (T, m)\<close> and
+    \<open>clauses_to_update T = {#}\<close> and
+    confl: \<open>\<not> brk \<longrightarrow> get_conflict T = None\<close>
+    using inv unfolding cdcl_twl_stgy_restart_prog_inv_def by fast+
+  have
+    cdcl_o: \<open>cdcl_twl_o\<^sup>*\<^sup>* S' U\<close> and
+    conflict_U: \<open>get_conflict U \<noteq> None \<Longrightarrow> count_decided (get_trail U) = 0\<close> and
+    brk'_no_step: \<open>brk' \<Longrightarrow> final_twl_state U\<close> and
+    struct_invs_U: \<open>twl_struct_invs U\<close> and
+    stgy_invs_U: \<open>twl_stgy_invs U\<close> and
+    clss_to_upd_U: \<open>clauses_to_update U = {#}\<close> and
+    lits_to_upd_U: \<open>\<not> brk' \<longrightarrow> literals_to_update U \<noteq> {#}\<close> and
+    confl_U: \<open>\<not> brk' \<longrightarrow> get_conflict U = None\<close>
+    using other_inv unfolding final_twl_state_def by fast+
+
+  have \<open>cdcl_twl_stgy\<^sup>*\<^sup>* T U\<close>
+    by (meson \<open>cdcl_twl_o\<^sup>*\<^sup>* S' U\<close> assms(5) rtranclp_cdcl_twl_cp_stgyD rtranclp_cdcl_twl_o_stgyD
+        rtranclp_trans)
+  have
+    twl_restart_after_restart:
+      \<open>cdcl_twl_stgy_restart (T, m) (V, Suc m)\<close> and
+    rtranclp_twl_restart_after_restart:
+      \<open>cdcl_twl_stgy_restart\<^sup>*\<^sup>* (S, 0) (V, m + 1)\<close> and
+    cdcl_twl_stgy_restart_with_leftovers_after_restart:
+      \<open>cdcl_twl_stgy_restart_with_leftovers (S, 0) (V, m + 1)\<close> and
+    cdcl_twl_stgy_restart_with_leftovers_after_restart_T_V:
+      \<open>cdcl_twl_stgy_restart_with_leftovers (T, m) (V, Suc m)\<close> and
+    cdcl_twl_stgy_restart_with_leftovers1_after_restart:
+      \<open>cdcl_twl_stgy_restart_with_leftovers1 (T, m) (V, Suc m)\<close>
+    if
+      f: \<open>True \<longrightarrow> f (snd (U, m)) < size (get_learned_clss (fst (U, m)))\<close> and
+      res: \<open>cdcl_twl_restart U V\<close> and
+      [simp]: \<open>brk' = False\<close>
+    for V
+  proof -
+    have \<open>S' \<noteq> U\<close>
+      using lits_to_update lits_to_upd_U by auto
+    then have \<open>cdcl_twl_o\<^sup>+\<^sup>+ S' U\<close>
+      using \<open>cdcl_twl_o\<^sup>*\<^sup>* S' U\<close> unfolding rtranclp_unfold by auto
+    then have st: \<open>cdcl_twl_stgy\<^sup>+\<^sup>+ T U\<close>
+      by (meson local.cp rtranclp_cdcl_twl_cp_stgyD rtranclp_tranclp_tranclp
+          tranclp_cdcl_twl_o_stgyD)
+
+    show twl_res_T_V: \<open>cdcl_twl_stgy_restart (T, m) (V, Suc m)\<close>
+      apply (rule cdcl_twl_stgy_restart.restart_step[of _ U])
+      subgoal by (rule st)
+      subgoal using f by simp
+      subgoal by (rule res)
+      done
+    show \<open>cdcl_twl_stgy_restart_with_leftovers (T, m) (V, Suc m)\<close>
+      unfolding cdcl_twl_stgy_restart_with_leftovers_def
+      by (rule exI[of _ \<open>V\<close>])(auto simp: twl_res_T_V)
+    show \<open>cdcl_twl_stgy_restart\<^sup>*\<^sup>* (S, 0) (V, m + 1)\<close>
+      using twl_res twl_res_T_V
+      unfolding cdcl_twl_stgy_restart_with_leftovers_def
+      by (auto dest: cdcl_twl_stgy_restart_cdcl_twl_stgy_cdcl_twl_stgy_restart)
+    then show  \<open>cdcl_twl_stgy_restart_with_leftovers (S, 0) (V, m + 1)\<close>
+      unfolding cdcl_twl_stgy_restart_with_leftovers_def apply -
+      by (rule exI[of _ V]) auto
+    show \<open>cdcl_twl_stgy_restart_with_leftovers1 (T, m) (V, Suc m)\<close>
+      using twl_res_T_V
+      unfolding cdcl_twl_stgy_restart_with_leftovers1_def
+      by fast
+  qed
+  have
+    rtranclp_twl_restart_after_restart_S_U:
+      \<open>cdcl_twl_stgy_restart_with_leftovers (S, 0) (U, m)\<close> and
+    rtranclp_twl_restart_after_restart_T_U:
+      \<open>cdcl_twl_stgy_restart_with_leftovers (T, m) (U, m)\<close>
+  proof -
+    obtain Ta where
+      S_Ta: \<open>cdcl_twl_stgy_restart\<^sup>*\<^sup>* (S, 0) (Ta, snd (T, m))\<close>
+      \<open>cdcl_twl_stgy\<^sup>*\<^sup>* Ta (fst (T, m))\<close>
+      using twl_res unfolding cdcl_twl_stgy_restart_with_leftovers_def
+      by auto
+    then have \<open>cdcl_twl_stgy\<^sup>*\<^sup>* Ta (fst (U, m))\<close>
+      using \<open>cdcl_twl_stgy\<^sup>*\<^sup>* T U\<close> by auto
+    then show \<open>cdcl_twl_stgy_restart_with_leftovers (S, 0) (U, m)\<close>
+      using S_Ta unfolding cdcl_twl_stgy_restart_with_leftovers_def
+      by fastforce
+    show \<open>cdcl_twl_stgy_restart_with_leftovers (T, m) (U, m)\<close>
+      using \<open>cdcl_twl_stgy\<^sup>*\<^sup>* T U\<close> unfolding cdcl_twl_stgy_restart_with_leftovers_def
+      by fastforce
+  qed
+  have
+    rtranclp_twl_restart_after_restart_brk:
+      \<open>cdcl_twl_stgy_restart_with_leftovers (S, 0) (U, m)\<close>
+    if
+      [simp]: \<open>brk' = True\<close>
+  proof -
+    have \<open>full1 cdcl_twl_stgy T U \<or> T = U \<or> get_conflict U \<noteq> None\<close>
+      using brk'_no_step \<open>cdcl_twl_stgy\<^sup>*\<^sup>* T U\<close>
+      unfolding rtranclp_unfold full1_def final_twl_state_def by auto
+    then consider
+        (step) \<open>cdcl_twl_stgy_restart (T, m) (U, m)\<close> |
+        (TU) \<open>T = U\<close> |
+        (final) \<open>get_conflict U \<noteq> None\<close>
+      by (auto dest!: cdcl_twl_stgy_restart.intros)
+    then show \<open>cdcl_twl_stgy_restart_with_leftovers (S, 0) (U, m)\<close>
+    proof cases
+      case step
+      then show ?thesis
+        using twl_res unfolding cdcl_twl_stgy_restart_with_leftovers_def
+        using cdcl_twl_stgy_restart_cdcl_twl_stgy_cdcl_twl_stgy_restart2[of T m U] apply -
+        by (rule exI[of _ U]) (fastforce dest!: )
+    next
+      case [simp]: TU
+      then show ?thesis
+        using twl_res unfolding cdcl_twl_stgy_restart_with_leftovers_def
+        using cdcl_twl_stgy_restart_cdcl_twl_stgy_cdcl_twl_stgy_restart2[of T m U] apply -
+        by fastforce
+    next
+      case final
+      then show ?thesis
+        using twl_res \<open>cdcl_twl_stgy\<^sup>*\<^sup>* T U\<close>  unfolding cdcl_twl_stgy_restart_with_leftovers_def
+        using cdcl_twl_stgy_restart_cdcl_twl_stgy_cdcl_twl_stgy_restart2[of T m U] apply -
+        by fastforce
+    qed
+  qed
+  have cdcl_twl_stgy_restart_with_leftovers1_T_U:
+    \<open>cdcl_twl_stgy_restart_with_leftovers1 (T, m) (U, m) \<longleftrightarrow> T \<noteq> U\<close>
+  proof -
+    have \<open>cdcl_twl_stgy\<^sup>+\<^sup>+ T U \<or> T = U\<close>
+      using \<open>cdcl_twl_stgy\<^sup>*\<^sup>* T U\<close> unfolding rtranclp_unfold by auto
+    then show ?thesis
+      using wf_not_refl[OF wf_cdcl_twl_stgy_restart, of \<open>(U, m)\<close>]
+      using wf_not_refl[OF tranclp_wf_cdcl_twl_stgy, of \<open>U\<close>]
+        struct_invs_U
+      unfolding cdcl_twl_stgy_restart_with_leftovers1_def by auto
+  qed
+  have brk'_eq: \<open>\<not>cdcl_twl_stgy_restart_with_leftovers1 (T, m) (U, m) \<Longrightarrow> brk'\<close>
+    using cdcl_o lits_to_upd_U lits_to_update local.cp
+    unfolding cdcl_twl_stgy_restart_with_leftovers1_def
+    unfolding rtranclp_unfold
+    by (auto dest!: tranclp_cdcl_twl_o_stgyD tranclp_cdcl_twl_cp_stgyD
+        simp: rtranclp_unfold
+        dest: rtranclp_tranclp_tranclp tranclp_trans)
+
+  have H[simp]: \<open>brk = False\<close> \<open>ebrk = False\<close>
+    using cond by auto
+  show ?B
+    unfolding restart_prog_def restart_required_def
+    apply (refine_vcg; remove_dummy_vars)
+    subgoal using struct_invs_U stgy_invs_U confl_U
+      unfolding restart_prog_pre_def cdcl_twl_stgy_restart_prog_inv_def H by fast
+    subgoal
+      unfolding cdcl_twl_stgy_restart_prog_inv_def
+      apply (intro conjI)
+      subgoal by (rule struct_invs')
+      subgoal by (rule stgy_invs)
+      subgoal unfolding H by fast
+      subgoal by (rule cdcl_twl_stgy_restart_with_leftovers_after_restart) simp_all
+      subgoal by (rule res_no_clss_to_upd)
+      subgoal by (simp add: res_no_confl)
+    done
+    subgoal
+     using cdcl_twl_stgy_restart_with_leftovers1_T_U brk'_eq struct_invs_T
+     by (simp add: clss_to_upd_U confl_U rtranclp_twl_restart_after_restart_S_U
+        stgy_invs_U struct_invs_U twl_restart_ops.cdcl_twl_stgy_restart_prog_inv_def
+	cdcl_twl_stgy_restart_with_leftovers1_after_restart)
+    subgoal
+     using cdcl_twl_stgy_restart_with_leftovers1_T_U brk'_eq
+     by (auto simp: twl_restart_after_restart struct_invs_S struct_invs_T
+	cdcl_twl_stgy_restart_with_leftovers_after_restart_T_V struct_invs_U
+	rtranclp_twl_restart_after_restart_brk rtranclp_twl_restart_after_restart_T_U
+	cdcl_twl_stgy_restart_with_leftovers1_after_restart
+	brk'_no_step clss_to_upd_U restart_prog_pre_def rtranclp_twl_restart_after_restart_S_U
+	twl_restart_ops.cdcl_twl_stgy_restart_prog_inv_def)
+    subgoal
+     using cdcl_twl_stgy_restart_with_leftovers1_T_U brk'_eq
+     by (auto simp: twl_restart_after_restart struct_invs_S struct_invs_T
+	cdcl_twl_stgy_restart_with_leftovers_after_restart_T_V struct_invs_U
+	rtranclp_twl_restart_after_restart_brk rtranclp_twl_restart_after_restart_T_U
+	cdcl_twl_stgy_restart_with_leftovers1_after_restart)
     done
 qed
 
@@ -325,6 +539,113 @@ proof -
     subgoal by fast
     subgoal by (rule restart_prog_spec[unfolded cdcl_twl_stgy_restart_prog_inv_def])
     subgoal by (rule final_prop[unfolded cdcl_twl_stgy_restart_prog_inv_def])
+    done
+qed
+
+definition cdcl_twl_stgy_restart_prog_early :: "'v twl_st \<Rightarrow> 'v twl_st nres" where
+  \<open>cdcl_twl_stgy_restart_prog_early S\<^sub>0 =
+  do {
+    (ebrk, brk, T, n) \<leftarrow> WHILE\<^sub>T\<^bsup>\<lambda>(ebrk, brk, T, n). cdcl_twl_stgy_restart_prog_inv S\<^sub>0 brk T n\<^esup>
+      (\<lambda>(ebrk, brk, _). \<not>brk \<and> \<not>ebrk)
+      (\<lambda>(ebrk, brk, S, n).
+      do {
+        T \<leftarrow> unit_propagation_outer_loop S;
+        (brk, T) \<leftarrow> cdcl_twl_o_prog T;
+        (T, n) \<leftarrow> restart_prog T n brk;
+	ebrk \<leftarrow> RES UNIV;
+        RETURN (ebrk, brk, T, n)
+      })
+      (False, False, S\<^sub>0, 0);
+    if \<not>brk then do {
+      (brk, T, _) \<leftarrow> WHILE\<^sub>T\<^bsup>\<lambda>(brk, T, n). cdcl_twl_stgy_restart_prog_inv S\<^sub>0 brk T n\<^esup>
+	(\<lambda>(brk, _). \<not>brk)
+	(\<lambda>(brk, S, n).
+	do {
+	  T \<leftarrow> unit_propagation_outer_loop S;
+	  (brk, T) \<leftarrow> cdcl_twl_o_prog T;
+	  (T, n) \<leftarrow> restart_prog T n brk;
+	  RETURN (brk, T, n)
+	})
+	(False, T, n);
+      RETURN T
+    }
+    else RETURN T
+  }\<close>
+
+lemma (in twl_restart) cdcl_twl_stgy_prog_early_spec:
+  assumes \<open>twl_struct_invs S\<close> and \<open>twl_stgy_invs S\<close> and \<open>clauses_to_update S = {#}\<close> and
+    \<open>get_conflict S = None\<close>
+  shows
+    \<open>cdcl_twl_stgy_restart_prog_early S \<le> SPEC(\<lambda>T. \<exists>n. cdcl_twl_stgy_restart_with_leftovers (S, 0) (T, n) \<and>
+        final_twl_state T)\<close>
+    (is \<open>_ \<le> SPEC(\<lambda>T. ?P T)\<close>)
+proof -
+  have final_prop: \<open>?P T\<close>
+    if
+     inv: \<open>case (brk, T, n) of  (brk, T, m) \<Rightarrow> cdcl_twl_stgy_restart_prog_inv S brk T m\<close> and
+      \<open>\<not> (case (brk, T, n) of (brk, uu_) \<Rightarrow> \<not> brk)\<close>
+    for brk T n
+  proof -
+    have
+      \<open>brk\<close> and
+      \<open>twl_struct_invs T\<close> and
+      \<open>twl_stgy_invs T\<close> and
+      ns: \<open>final_twl_state T\<close> and
+      twl_left_overs: \<open>cdcl_twl_stgy_restart_with_leftovers (S, 0) (T, n)\<close> and
+      \<open>clauses_to_update T = {#}\<close>
+      using that unfolding cdcl_twl_stgy_restart_prog_inv_def by auto
+    obtain S' where
+       st: \<open>cdcl_twl_stgy_restart\<^sup>*\<^sup>* (S, 0) (S', n)\<close> and
+       S'_T: \<open>cdcl_twl_stgy\<^sup>*\<^sup>* S' T\<close>
+      using twl_left_overs unfolding cdcl_twl_stgy_restart_with_leftovers_def by auto
+    then show ?thesis
+      using ns unfolding cdcl_twl_stgy_restart_with_leftovers_def apply -
+      apply (rule_tac x=n in exI)
+      apply (rule conjI)
+      subgoal by (rule_tac x=S' in exI) auto
+      subgoal by auto
+      done
+  qed
+  show ?thesis
+    supply RETURN_as_SPEC_refine[refine2 del]
+    unfolding cdcl_twl_stgy_restart_prog_early_def full_def
+    apply (refine_vcg
+        WHILEIT_rule[where
+           R = \<open>{((ebrk, brkT, T, n), (ebrk, brkS, S, m)).
+                     twl_struct_invs S \<and> cdcl_twl_stgy_restart_with_leftovers1 (S, m) (T, n)} \<union>
+                {((ebrkT, brkT, T), (ebrkS, brkS, S)). S = T \<and> (ebrkT \<or> brkT) \<and> (\<not>brkS \<and> \<not>ebrkS)}\<close>]
+       WHILEIT_rule[where
+           R = \<open>{((brkT, T, n), (brkS, S, m)).
+                     twl_struct_invs S \<and> cdcl_twl_stgy_restart_with_leftovers1 (S, m) (T, n)} \<union>
+                {((brkT, T), (brkS, S)). S = T \<and> brkT \<and> \<not>brkS}\<close>];
+        remove_dummy_vars)
+    subgoal by (rule wf_cdcl_twl_stgy_restart_measure_early)
+    subgoal using assms unfolding cdcl_twl_stgy_restart_prog_inv_def
+      by (fast intro: cdcl_twl_stgy_restart_with_leftovers_refl)
+    subgoal unfolding cdcl_twl_stgy_restart_prog_inv_def by fast
+    subgoal unfolding cdcl_twl_stgy_restart_prog_inv_def by fast
+    subgoal unfolding cdcl_twl_stgy_restart_prog_inv_def by fast
+    subgoal unfolding cdcl_twl_stgy_restart_prog_inv_def by fast
+    subgoal unfolding cdcl_twl_stgy_restart_prog_inv_def
+      by (simp add: no_step_cdcl_twl_cp_no_step_cdcl\<^sub>W_cp)
+    subgoal by fast
+    subgoal for ebrk brk T m x ac bc
+      by (rule restart_prog_early_spec)
+    subgoal by (rule wf_cdcl_twl_stgy_restart_measure)
+    subgoal by fast
+    subgoal unfolding cdcl_twl_stgy_restart_prog_inv_def by fast
+    subgoal unfolding cdcl_twl_stgy_restart_prog_inv_def by fast
+    subgoal unfolding cdcl_twl_stgy_restart_prog_inv_def by fast
+    subgoal unfolding cdcl_twl_stgy_restart_prog_inv_def by fast
+    subgoal unfolding cdcl_twl_stgy_restart_prog_inv_def
+      by (simp add: no_step_cdcl_twl_cp_no_step_cdcl\<^sub>W_cp)
+    subgoal by fast
+    subgoal unfolding cdcl_twl_stgy_restart_prog_inv_def
+      by (rule restart_prog_spec[unfolded cdcl_twl_stgy_restart_prog_inv_def])
+    subgoal unfolding cdcl_twl_stgy_restart_prog_inv_def
+      by (rule final_prop[unfolded cdcl_twl_stgy_restart_prog_inv_def])
+    subgoal unfolding cdcl_twl_stgy_restart_prog_inv_def
+      by auto
     done
 qed
 
